functions to create and free a verifier state

steel/Veritas.Steel.VCache.fst
@@ -5,6 +5,8 @@ let vcache_create n =
   let h = get () in //TODO: need this unnecessarily
   malloc None (C.uint16_to_uint32 n)
 
+let free #n v = Steel.Array.free v
+
 let vcache_get_record vst s =
   index vst (C.uint16_to_uint32 s)
 
